# Math128A: Sample Final Exam

This is a closed book exam, with the exception of a one-page cheat sheet on one side only. You are allowed to cite any results, up to Section 6.6 but excluding those in the exercises, from the textbook. Results from anywhere else will need to be justified. Completely correct answers given without justification will receive little credit. Partial solutions will get partial credit.

---

1.  Let $h>0$. Develop a finite difference method to approximate the derivative $f^{\prime}(x_{0})$ using function values $f(x_{0}-h), f(x_{0}+2h)$.
    (a) What is the order of your method?
    (b) Turn your method into a second order method with extrapolation.
***Solution*:** 
We seek an approximation $f'(x_0) \approx c_1 f(x_0-h) + c_2 f(x_0+2h)$.
Using Taylor expansions around $x_0$:
$f(x_0-h) = f(x_0) - h f'(x_0) + \frac{h^2}{2} f''(x_0) + O(h^3)$
$f(x_0+2h) = f(x_0) + 2h f'(x_0) + 2h^2 f''(x_0) + O(h^3)$

Substituting into the approximation:
$c_1 f(x_0-h) + c_2 f(x_0+2h) = (c_1+c_2)f(x_0) + (-c_1+2c_2)h f'(x_0) + (\frac{c_1}{2}+2c_2)h^2 f''(x_0) + O(h^3)$.
>[!Note]
>The key is to construct the equations based on this approximation

To approximate $f'(x_0)$, we set:
1.  $c_1+c_2 = 0 \implies c_2 = -c_1$
2.  $(-c_1+2c_2)h = 1$

Solving this system:
$(-c_1-2c_1)h = 1 \implies -3c_1h = 1 \implies c_1 = -\frac{1}{3h}$.
Thus, $c_2 = \frac{1}{3h}$.
The finite difference formula is $N(h) = \frac{f(x_0+2h) - f(x_0-h)}{3h}$.

**(a) Order of the method**

To find the order, we expand $N(h)$ using Taylor series for $f(x_0-h)$ and $f(x_0+2h)$ up to higher order terms:
$f(x_0-h) = f(x_0) - hf'(x_0) + \frac{h^2}{2}f''(x_0) - \frac{h^3}{6}f'''(x_0) + O(h^4)$
$f(x_0+2h) = f(x_0) + 2hf'(x_0) + 2h^2f''(x_0) + \frac{4h^3}{3}f'''(x_0) + O(h^4)$

$N(h) = \frac{1}{3h} \left[ (f(x_0+2h) - f(x_0)) - (f(x_0-h) - f(x_0)) \right]$
$N(h) = \frac{1}{3h} \left[ (2hf'(x_0) + 2h^2f''(x_0) + \frac{4h^3}{3}f'''(x_0)) - (-hf'(x_0) + \frac{h^2}{2}f''(x_0) - \frac{h^3}{6}f'''(x_0)) + O(h^4) \right]$
$N(h) = \frac{1}{3h} \left[ 3hf'(x_0) + \left(2-\frac{1}{2}\right)h^2f''(x_0) + \left(\frac{4}{3}+\frac{1}{6}\right)h^3f'''(x_0) + O(h^4) \right]$
$N(h) = f'(x_0) + \frac{1}{2}hf''(x_0) + \frac{1}{2}h^2f'''(x_0) + O(h^3)$.

The local truncation error is $LTE = f'(x_0) - N(h) = -\frac{h}{2}f''(x_0) - \frac{h^2}{2}f'''(x_0) + O(h^3)$.
The leading error term is $-\frac{h}{2}f''(x_0)$, so the method is first order ($O(h)$).

>[!Caution]
>Unlike in ODEs, the LTE here doesn't need to be divided by $h$, so keep this in mind!

**(b) Turn your method into a second order method with extrapolation**

The error expansion is $f'(x_0) = N(h) + K_1 h + K_2 h^2 + O(h^3)$, where $K_1 = -\frac{1}{2}f''(x_0)$.
Richardson extrapolation for a first-order method **uses $N(h)$ and $N(h/2)$.** 
The formula for the extrapolated value $N_2(h)$ is:
- $N_2(h) = 2N(h/2) - N(h)$.
- $N(h/2) = \frac{f(x_0+2(h/2)) - f(x_0-(h/2))}{3(h/2)} = \frac{f(x_0+h) - f(x_0-h/2)}{3h/2}$.

Substituting into $N_2(h)$:
$N_2(h) = 2 \left( \frac{f(x_0+h) - f(x_0-h/2)}{3h/2} \right) - \left( \frac{f(x_0+2h) - f(x_0-h)}{3h} \right)$
$N_2(h) = \frac{4(f(x_0+h) - f(x_0-h/2))}{3h} - \frac{f(x_0+2h) - f(x_0-h)}{3h}$
$N_2(h) = \frac{1}{3h} \left( 4f(x_0+h) - 4f(x_0-h/2) - f(x_0+2h) + f(x_0-h) \right)$.
This method $N_2(h)$ is second order ($O(h^2)$).
>[!note]
>The key idea here is to extrapolate using $N\left( \frac{h}{2} \right)$ to eliminate $K_{1}$, then we can get the key formula: $N_{2}(h)  = 2N\left( \frac{h}{2} \right)-N(h)$.
---

---
2.  Consider the iteration
    $$x_{k+1}=-(\alpha-1)x_k+\frac{1}{2}x_k^2,\quad k=0,1,\cdots,$$
    where $0<\alpha\leq1$ is given. Assume that the iteration converges to $0$ for all initial points $x_0$. What is the order of convergence for $0<\alpha<1$? What is the order of convergence for $\alpha=1$?

***Solution:***
Let the fixed-point iteration function be $g(x)$. The iteration is given by $x_{k+1} = g(x_k)$, where
$$g(x) = -(\alpha-1)x + \frac{1}{2}x^2 = (1-\alpha)x + \frac{1}{2}x^2.$$
We are given that the iteration converges to the fixed point $x^*=0$. The order of convergence is determined by the derivatives of $g(x)$ evaluated at $x^*=0$.

First, calculate the derivatives of $g(x)$:
$$g'(x) = \frac{d}{dx}\left((1-\alpha)x + \frac{1}{2}x^2\right) = (1-\alpha) + x$$
$$g''(x) = \frac{d}{dx}((1-\alpha) + x) = 1$$

Next, evaluate these derivatives at the fixed point $x^*=0$:
$$g'(0) = (1-\alpha) + 0 = 1-\alpha$$
$$g''(0) = 1$$

We now analyze the two cases for $\alpha$:

**Case 1: $0 < \alpha < 1$**

In this case, $1-\alpha$ satisfies $0 < 1-\alpha < 1$.
Therefore, $g'(0) = 1-\alpha$.
Since $0 < g'(0) < 1$, specifically $g'(0) \neq 0$.
When $g'(x^*) \neq 0$ and $|g'(x^*)| < 1$, the convergence is linear.
Thus, for $0 < \alpha < 1$, the order of convergence is **1 (linear)**.

>[!note]
>The key here is to think of this equation: $\lim_{ k \to \infty }\left\lvert  \frac{x_{k+1}-x^*}{x_{k}-x^*} \right\rvert = \lvert g'(x^*) \rvert$, and this can be derived by Taylor expansion.

**Case 2: $\alpha = 1$**

In this case, $1-\alpha = 1-1 = 0$.
Therefore, $g'(0) = 0$.
Since $g'(0) = 0$, the convergence is faster than linear. We look at the next derivative:
$g''(0) = 1$.
Since $g'(0) = 0$ and $g''(0) = 1 \neq 0$, the theory of fixed-point iteration states that the convergence is quadratic.
Thus, for $\alpha = 1$, the order of convergence is **2 (quadratic)**.

To summarize:
* For $0 < \alpha < 1$, the order of convergence is 1 (linear).
* For $\alpha = 1$, the order of convergence is 2 (quadratic).

>[!caution]
>You need to keep in mind the definition of the order of convergence and the rate of convergence!

---

3.  Determine the constants $C$ and $x_0$ so that the following quadrature
    $$\int_{-\infty}^{\infty}e^{-|x|}\:f(x)\:dx\approx C\:f(x_0)$$
    is exact for $f(x)=1$, $f(x)=x$.

***Solutions:***
The problem is to determine the constants $C$ and $x_0$ such that the quadrature rule
$$\int_{-\infty}^{\infty}e^{-|x|}f(x)dx \approx C f(x_0)$$
is exact for the functions $f(x)=1$ and $f(x)=x$.

We enforce this exactness for each function.

**Case 1: $f(x)=1$**
The exact integral is:
$$ I_1 = \int_{-\infty}^{\infty} e^{-|x|} (1) dx $$
Since $e^{-|x|}$ is an even function, we have:
$$ I_1 = 2 \int_{0}^{\infty} e^{-x} dx = 2 \left[-e^{-x}\right]_{0}^{\infty} = 2 (0 - (-e^0)) = 2(1) = 2 $$
The approximation is:
$$ A_1 = C \cdot f(x_0) = C \cdot 1 = C $$
For the rule to be exact, $I_1 = A_1$, so:
$$ C = 2 \tag{1} $$

**Case 2: $f(x)=x$**
The exact integral is:
$$ I_2 = \int_{-\infty}^{\infty} e^{-|x|} x dx $$
The integrand $g(x) = x e^{-|x|}$ is an odd function, as $g(-x) = (-x)e^{-|-x|} = -x e^{-|x|} = -g(x)$. The integral of an odd function over a symmetric interval $(-\infty, \infty)$ is 0.
$$ I_2 = 0 $$
The approximation is:
$$ A_2 = C \cdot f(x_0) = C \cdot x_0 $$
For the rule to be exact, $I_2 = A_2$, so:
$$ C x_0 = 0 \tag{2} $$

**Solving for the constants**
We have the system of equations:
1.  $C = 2$
2.  $C x_0 = 0$

Substitute $C=2$ from (1) into (2):
$$ 2 x_0 = 0 $$
$$ x_0 = 0 $$

Therefore, the constants are $C=2$ and $x_0=0$.

---

4.  By performing Gaussian elimination with partial pivoting, find the permutation matrix $P$, the lower triangular matrix $L$ with 1â€™s on its diagonal, and the upper triangular matrix $U$ so that
    $$PA=LU,\quad\text{where}\quad A=\begin{pmatrix}0&1&1\\1&-2&-1\\1&-1&1\end{pmatrix}.$$
***Solutions:***

We want to find matrices $P, L, U$ such that $PA=LU$ for the given matrix $A$ using Gaussian elimination with partial pivoting. $L$ must have 1s on its diagonal.

Initial state:
$$ A = \begin{pmatrix} 0 & 1 & 1 \\ 1 & -2 & -1 \\ 1 & -1 & 1 \end{pmatrix}, \quad P = \begin{pmatrix} 1 & 0 & 0 \\ 0 & 1 & 0 \\ 0 & 0 & 1 \end{pmatrix}, \quad L = \begin{pmatrix} 1 & 0 & 0 \\ 0 & 1 & 0 \\ 0 & 0 & 1 \end{pmatrix} $$

**Step 1: Process column 1 ($k=1$)**

* **Partial Pivoting:**
    The first column of $A$ is $\begin{pmatrix} 0 \\ 1 \\ 1 \end{pmatrix}$. The element with the largest absolute value is 1, found in row 2 (element $a_{21}=1$) and row 3 (element $a_{31}=1$). We choose the one with the smaller row index, so we select row 2 as the pivot row.
    Swap row 1 and row 2.
    -   Swap rows 1 and 2 of $A$:
        $$ A \leftarrow \begin{pmatrix} 1 & -2 & -1 \\ 0 & 1 & 1 \\ 1 & -1 & 1 \end{pmatrix} $$
    -   Swap rows 1 and 2 of $P$:
        $$ P \leftarrow \begin{pmatrix} 0 & 1 & 0 \\ 1 & 0 & 0 \\ 0 & 0 & 1 \end{pmatrix} $$
    -   Swap $L_{1,j}$ with $L_{2,j}$ for $j < 1$. There are no such columns, so $L$ is unchanged by this rule for existing entries.

* **Elimination:**
    The pivot element is $a_{11}=1$.
    -   For row 2 ($i=2$): The element $a_{21}=0$. The multiplier $m_{21} = a_{21}/a_{11} = 0/1 = 0$.
        Store $L_{21}=0$. Row 2 remains $R_2 \leftarrow R_2 - 0 \cdot R_1$.
        The matrix $A$ is unchanged here.
    -   For row 3 ($i=3$): The element $a_{31}=1$. The multiplier $m_{31} = a_{31}/a_{11} = 1/1 = 1$.
        Store $L_{31}=1$. Perform $R_3 \leftarrow R_3 - m_{31} R_1 = R_3 - 1 \cdot R_1$:
        $$ R_3 = (1, -1, 1) - (1, -2, -1) = (1-1, -1-(-2), 1-(-1)) = (0, 1, 2) $$
    After elimination for column 1, the matrices are:
    $$ A \leftarrow \begin{pmatrix} 1 & -2 & -1 \\ 0 & 1 & 1 \\ 0 & 1 & 2 \end{pmatrix}, \quad L \leftarrow \begin{pmatrix} 1 & 0 & 0 \\ 0 & 1 & 0 \\ 1 & 0 & 1 \end{pmatrix} $$
    $P$ remains $\begin{pmatrix} 0 & 1 & 0 \\ 1 & 0 & 0 \\ 0 & 0 & 1 \end{pmatrix}$.

**Step 2: Process column 2 ($k=2$)**

* **Partial Pivoting:**
    Consider elements below or at the diagonal in column 2: $a_{22}=1, a_{32}=1$. The maximum absolute value is 1. The current pivot element $a_{22}=1$ is suitable. No row swap is needed.
    $P, A, L$ (sub-diagonal part of column 1) remain unchanged from this sub-step.

* **Elimination:**
    The pivot element is $a_{22}=1$.
    -   For row 3 ($i=3$): The element $a_{32}=1$. The multiplier $m_{32} = a_{32}/a_{22} = 1/1 = 1$.
        Store $L_{32}=1$. Perform $R_3 \leftarrow R_3 - m_{32} R_2 = R_3 - 1 \cdot R_2$:
        $$ R_3 = (0, 1, 2) - (0, 1, 1) = (0-0, 1-1, 2-1) = (0, 0, 1) $$
    After elimination for column 2, the matrix $A$ has become $U$:
    $$ U = A \leftarrow \begin{pmatrix} 1 & -2 & -1 \\ 0 & 1 & 1 \\ 0 & 0 & 1 \end{pmatrix} $$
    The matrix $L$ is now fully determined:
    $$ L \leftarrow \begin{pmatrix} 1 & 0 & 0 \\ 0 & 1 & 0 \\ 1 & 1 & 1 \end{pmatrix} $$
    $P$ remains $\begin{pmatrix} 0 & 1 & 0 \\ 1 & 0 & 0 \\ 0 & 0 & 1 \end{pmatrix}$.

**Final Result:**
The decomposition is:
$$ P = \begin{pmatrix} 0 & 1 & 0 \\ 1 & 0 & 0 \\ 0 & 0 & 1 \end{pmatrix} $$
$$ L = \begin{pmatrix} 1 & 0 & 0 \\ 0 & 1 & 0 \\ 1 & 1 & 1 \end{pmatrix} $$
$$ U = \begin{pmatrix} 1 & -2 & -1 \\ 0 & 1 & 1 \\ 0 & 0 & 1 \end{pmatrix} $$

Verification (optional):
$PA = \begin{pmatrix} 0 & 1 & 0 \\ 1 & 0 & 0 \\ 0 & 0 & 1 \end{pmatrix} \begin{pmatrix} 0 & 1 & 1 \\ 1 & -2 & -1 \\ 1 & -1 & 1 \end{pmatrix} = \begin{pmatrix} 1 & -2 & -1 \\ 0 & 1 & 1 \\ 1 & -1 & 1 \end{pmatrix}$
$LU = \begin{pmatrix} 1 & 0 & 0 \\ 0 & 1 & 0 \\ 1 & 1 & 1 \end{pmatrix} \begin{pmatrix} 1 & -2 & -1 \\ 0 & 1 & 1 \\ 0 & 0 & 1 \end{pmatrix} = \begin{pmatrix} 1 & -2 & -1 \\ 0 & 1 & 1 \\ 1 & -1 & 1 \end{pmatrix}$
Since $PA=LU$, the decomposition is correct.

---

5.  Given an initial value ODE
    $$y'=f(t,y),\quad\mathrm{for}\quad a\leq t\leq b,\quad y(a)=\alpha.\tag{1}$$
    Consider the multi-step method for solving (1)
    $$w_{k+1}=-4w_{k}+5w_{k-1}+h\left(\gamma\:f(t_{k},w_{k})+\beta\:f(t_{k-1},w_{k-1})\right),\quad k=1,2,\cdots,N-1\tag{2}$$
    with starting values $w_{0},w_{1}$.
    (a) Choose the constants $\gamma$ and $\beta$ so the method (2) is of 2nd order.

---

6.  Compute $\mathrm{det}(A)$ with $A=\begin{pmatrix}1&2&0\\2&1&3\\0&4&\alpha\end{pmatrix}$. For which values of $\alpha$ is $\operatorname*{det}(A)=0$?

---

7.  Determine the exact conditions on the coefficients $a,b,c,d,e$ under which the following function is a cubic spline (i.e., $f\in C^{2}(-\infty,\infty)$):
    $$f(x)=\begin{cases}a(x-1)^2+b\:x^3,&\text{if }x\in(-\infty,0],\\c(x-1)^2,&\text{if }x\in[0,2],\\d(x-2)^3+e(x-1)^2,&\text{if }x\in[2,\infty).\end{cases}$$

---

8.  Does the function $f(t, y) = t^{2}y^{3}$ satisfy the Lipschitz condition on the domain
    $$\mathcal{D}\stackrel{\text{def}}{=}\{(t,y)\mid0\leq t\leq1,\:-\infty<y<\infty\}?$$